common/theories/LoopChecking/ModelValuation.v
@@ -9,7 +9,7 @@
 
       Definition clause_sem (cl : clause) : Prop :=
         let '(prems, concl) := cl in
-        le (interp_expr concl) (interp_prems prems).
+        le (interp_expr concl) (interp_nes prems).
 
       Definition clauses_sem (cls : clauses) : Prop :=
         Clauses.For_all clause_sem cls.
@@ -37,7 +37,7 @@
       rewrite /add_expr; cbn.
       rewrite -add_distr => le. now apply (le_add (n:=n)) in le.
     - intros V clsm. cbn.
-      rewrite interp_prems_singleton.
+      rewrite interp_nes_singleton.
       cbn. red. rewrite -!add_distr. rewrite -add_join.
       now rewrite join_sub.
   Qed.
@@ -54,13 +54,13 @@
     induction 1.
     - intros v clls. red.
       destruct concl0 as [concl k].
-      have hge := interp_prems_ge (SL := Zsemilattice) v prems _ H.
+      have hge := interp_nes_ge (SL := Zsemilattice) v prems _ H.
       cbn in *. by lia.
     - move=> V Hcls.
       move: {IHentails} (IHentails _ Hcls).
       unfold clause_sem. unfold ge => hyp.
-      etransitivity; tea. rewrite interp_prems_add.
-      rewrite interp_prems_add in hyp.
+      etransitivity; tea. rewrite interp_nes_add.
+      rewrite interp_nes_add in hyp.
       eapply in_pred_closure_entails in H; tea.
       move: H; rewrite /clause_sem. unfold ge.
       have ssub := clauses_sem_subset (SL := Zsemilattice) H1 V.
@@ -69,13 +69,13 @@
 
   Lemma clauses_sem_entails_all {cls prems concl} :
     cls ⊢a prems → concl ->
-    (forall V, clauses_sem V cls -> interp_prems V concl ≤ interp_prems V prems).
+    (forall V, clauses_sem V cls -> interp_nes V concl ≤ interp_nes V prems).
   Proof.
     intros ha V hcls.
     red in ha.
     move: ha.
     revert concl.
-    refine (@interp_prems_elim _ _ (fun concl z => _ -> z ≤ interp_prems V prems) V _ _ _).
+    refine (@interp_nes_elim _ _ (fun concl z => _ -> z ≤ interp_nes V prems) V _ _ _).
     - move=> le //=. move/(_ le).
       intros h; forward h by now apply LevelExprSet.singleton_spec.
       now have ent := (clauses_sem_entails h _ hcls).
